X1

NuBasicAbstractors.thy
@@ -6,7 +6,7 @@ begin
 
 text \<open>Basic \<nu>-abstractors\<close>
 
-text \<open>Examples for automatic property inference\<close>
+(* text \<open>Examples for automatic property inference\<close>
 schematic_goal [simplified]: "\<nu>Share (\<bool> \<nuFusion> \<nat>['b :: len] \<nuFusion> \<bool>) ?set ?sh" by (rule \<nu>intro)+
 (* schematic_goal [simplified]: "\<nu>Share N s f \<Longrightarrow> \<nu>Share (N \<nuFusion> N \<nuFusion> N) ?set ?sh" for N :: "('a::sharable_lrep, 'b) nu"
   including show_more1 by (blast intro: \<nu>intro Premise_I) *)
@@ -20,29 +20,88 @@ val tm = Thm.cprop_of @{thm th1}
 val th = Goal.init tm2
 val th2 = SOLVED' (Tactical.REPEAT o Tactic.ares_tac @{context} @{thms \<nu>share}) 1 th |> Seq.hd
 \<close>
-
+*)
 section \<open>Abstractors for specification\<close>
 
 subsubsection \<open>Refinement\<close>
 
 definition NuRefine :: " ('a :: lrep, 'b) nu \<Rightarrow> 'b set \<Rightarrow> ('a, 'b) nu " (infixl "\<nuRefine>" 80)
   where "N \<nuRefine> T = Nu (\<lambda>(p,x). x \<in> T \<and>(p \<nuLinkL> N \<nuLinkR> x))"
-notation NuRefine (infixl "\<where>" 10) and NuRefine (infixl "\<^bold>w\<^bold>h\<^bold>e\<^bold>r\<^bold>e" 10)
+
+notation NuRefine (infixl "<where>" 10) and NuRefine (infixl "\<^bold>w\<^bold>h\<^bold>e\<^bold>r\<^bold>e" 60)
+
 lemma [simp]: "p \<nuLinkL> N \<nuRefine> P \<nuLinkR> x \<longleftrightarrow> x \<in> P \<and> (p \<nuLinkL> N \<nuLinkR> x)" unfolding NuRefine_def by auto
 lemma [elim]: "x \<ratio> N \<nuRefine> P \<Longrightarrow> (x \<in> P \<Longrightarrow> x \<ratio> N \<Longrightarrow> C) \<Longrightarrow> C" unfolding Inhabited_def by auto
 lemma [\<nu>intro]: "(x \<in> P \<Longrightarrow> \<^bold>c\<^bold>a\<^bold>s\<^bold>t x \<tycolon> N \<longmapsto> Y \<^bold>m\<^bold>e\<^bold>a\<^bold>n\<^bold>w\<^bold>h\<^bold>i\<^bold>l\<^bold>e Q) \<Longrightarrow> \<^bold>c\<^bold>a\<^bold>s\<^bold>t x \<tycolon> N \<nuRefine> P \<longmapsto> Y \<^bold>m\<^bold>e\<^bold>a\<^bold>n\<^bold>w\<^bold>h\<^bold>i\<^bold>l\<^bold>e Q \<and>x \<in> P" unfolding Cast_def by auto
 lemma [\<nu>cast_overload E]: "\<^bold>c\<^bold>a\<^bold>s\<^bold>t x \<tycolon> (N \<^bold>w\<^bold>h\<^bold>e\<^bold>r\<^bold>e P) \<longmapsto> x \<tycolon> N \<^bold>m\<^bold>e\<^bold>a\<^bold>n\<^bold>w\<^bold>h\<^bold>i\<^bold>l\<^bold>e x \<in> P" unfolding Cast_def by auto
 lemma where_\<nu>cast: "\<^bold>p\<^bold>a\<^bold>r\<^bold>a\<^bold>m P \<Longrightarrow> \<^bold>p\<^bold>r\<^bold>e\<^bold>m\<^bold>i\<^bold>s\<^bold>e x \<in> P \<Longrightarrow> \<^bold>c\<^bold>a\<^bold>s\<^bold>t x \<tycolon> N \<longmapsto> x \<tycolon> (N \<^bold>w\<^bold>h\<^bold>e\<^bold>r\<^bold>e P)" unfolding Cast_def by auto
 
+lemma [\<nu>intro]: "\<^bold>p\<^bold>r\<^bold>e\<^bold>m\<^bold>i\<^bold>s\<^bold>e \<forall>x. P' x \<longrightarrow> P x \<Longrightarrow> \<^bold>p\<^bold>r\<^bold>e\<^bold>m\<^bold>i\<^bold>s\<^bold>e \<forall>x z. P' x \<and> x \<in> S \<and> (x \<ratio> N) \<longrightarrow> s z x \<in> S \<Longrightarrow> \<nu>Share N P s \<Longrightarrow> \<nu>Share (N \<^bold>w\<^bold>h\<^bold>e\<^bold>r\<^bold>e S) P' s"
+  unfolding \<nu>Share_def by (auto 0 3)
+lemma [\<nu>intro]: "\<^bold>p\<^bold>r\<^bold>e\<^bold>m\<^bold>i\<^bold>s\<^bold>e \<forall>x. x \<in> S \<and> (x \<ratio> N) \<longrightarrow> dp x \<in> S \<Longrightarrow> \<nu>Deprive N dp \<Longrightarrow> \<nu>Deprive (N \<^bold>w\<^bold>h\<^bold>e\<^bold>r\<^bold>e S) dp"
+  unfolding \<nu>Deprive_def by (auto 0 3)
+lemma [\<nu>intro]: "\<nu>CEqual N P eq \<Longrightarrow> \<nu>CEqual (N \<^bold>w\<^bold>h\<^bold>e\<^bold>r\<^bold>e S) P eq" unfolding \<nu>CEqual_def by auto
+lemma [\<nu>intro]: "\<nu>Ownership N ow \<Longrightarrow> \<nu>Ownership (N \<^bold>w\<^bold>h\<^bold>e\<^bold>r\<^bold>e S) ow" unfolding \<nu>Ownership_def by simp
+lemma [\<nu>intro]: "\<nu>ShrIdentical N sid \<Longrightarrow> \<nu>ShrIdentical (N \<^bold>w\<^bold>h\<^bold>e\<^bold>r\<^bold>e S) sid" unfolding \<nu>ShrIdentical_def by auto
+lemma [\<nu>intro]: "\<nu>Disposable \<tort_lbrace>x \<tycolon> N\<tort_rbrace> \<Longrightarrow> \<nu>Disposable \<tort_lbrace>x \<tycolon> (N \<^bold>w\<^bold>h\<^bold>e\<^bold>r\<^bold>e S)\<tort_rbrace>" unfolding \<nu>Disposable_def by simp
+
+subsubsection \<open>Down Lifting\<close>
+
+definition DownLift :: "(('a::lrep), 'b) nu \<Rightarrow> ('c \<Rightarrow> 'b) \<Rightarrow> ('a,'c) nu" (infixl "<down-lift>" 80)
+  where "DownLift N g = Nu (\<lambda>(p,x). p \<nuLinkL> N \<nuLinkR> g x)"
+
+lemma [simp]: "p \<nuLinkL> N <down-lift> g \<nuLinkR> x \<longleftrightarrow> p \<nuLinkL> N \<nuLinkR> g x" unfolding DownLift_def by simp
+lemma [elim]: "x \<ratio> N <down-lift> g \<Longrightarrow> (g x \<ratio> N \<Longrightarrow> C) \<Longrightarrow> C" unfolding Inhabited_def by simp
+
+subsubsection \<open>Up Lifting\<close>
+
+definition UpLift :: "(('a::lrep), 'c) nu \<Rightarrow> ('c \<Rightarrow> 'b) \<Rightarrow> ('a,'b) nu" (infixl "<up-lift>" 80)
+  where "UpLift N f = Nu (\<lambda>(p,x). \<exists>y. f y = x \<and> (p \<nuLinkL> N \<nuLinkR> y))"
+
+lemma [simp]: "p \<nuLinkL> N <up-lift> f \<nuLinkR> x \<longleftrightarrow> (\<exists>y. (f y = x) \<and> (p \<nuLinkL> N \<nuLinkR> y))" unfolding UpLift_def by simp
+lemma [elim]: "x \<ratio> N <up-lift> f \<Longrightarrow> (\<And>y. y \<ratio> N \<Longrightarrow> f y = x \<Longrightarrow> C) \<Longrightarrow> C" unfolding Inhabited_def by auto
+
+lemma [\<nu>intro]: "\<nu>Share "
+
+subsubsection \<open>Operator Some\<close>
+
 definition NuSome :: " ('a :: lrep, 'b) nu \<Rightarrow> ('a :: lrep, 'b set) nu " ("<some>")
   where "NuSome N = Nu (\<lambda>(p,S). \<exists>x. x \<in> S \<and> (p \<nuLinkL> N \<nuLinkR> x))"
 notation NuSome ("\<^bold>s\<^bold>o\<^bold>m\<^bold>e")
+
 lemma [simp]: "p \<nuLinkL> \<^bold>s\<^bold>o\<^bold>m\<^bold>e N \<nuLinkR> X \<longleftrightarrow> (\<exists>x. x \<in> X \<and> (p \<nuLinkL> N \<nuLinkR> x))" unfolding NuSome_def by auto
 lemma [elim]: "X \<ratio> ( \<^bold>s\<^bold>o\<^bold>m\<^bold>e N) \<Longrightarrow> (\<And>x. x \<in> X \<Longrightarrow> x \<ratio> N \<Longrightarrow> C) \<Longrightarrow> C" unfolding Inhabited_def by auto
-lemma [\<nu>intro]: "\<^bold>p\<^bold>r\<^bold>e\<^bold>m\<^bold>i\<^bold>s\<^bold>e X \<subseteq> X' \<Longrightarrow> \<^bold>c\<^bold>a\<^bold>s\<^bold>t X \<tycolon> (\<^bold>s\<^bold>o\<^bold>m\<^bold>e N) \<longmapsto> X' \<tycolon> (\<^bold>s\<^bold>o\<^bold>m\<^bold>e N)" unfolding Cast_def by auto
+lemma [\<nu>intro]: "\<^bold>p\<^bold>r\<^bold>e\<^bold>m\<^bold>i\<^bold>s\<^bold>e X \<subseteq> X' \<Longrightarrow> \<^bold>c\<^bold>a\<^bold>s\<^bold>t X \<tycolon> (\<^bold>s\<^bold>o\<^bold>m\<^bold>e N) \<longmapsto> X' \<tycolon> (\<^bold>s\<^bold>o\<^bold>m\<^bold>e N)" unfolding Cast_def by (auto 2 3)
 lemma [\<nu>intro]: "\<^bold>p\<^bold>r\<^bold>e\<^bold>m\<^bold>i\<^bold>s\<^bold>e x \<in> X \<Longrightarrow> \<^bold>c\<^bold>a\<^bold>s\<^bold>t x \<tycolon> N \<longmapsto> X \<tycolon> (\<^bold>s\<^bold>o\<^bold>m\<^bold>e N)" unfolding Cast_def by auto
 lemma someI_\<nu>cast: "\<^bold>p\<^bold>a\<^bold>r\<^bold>a\<^bold>m X \<Longrightarrow> \<^bold>p\<^bold>r\<^bold>e\<^bold>m\<^bold>i\<^bold>s\<^bold>e x \<in> X \<Longrightarrow> \<^bold>c\<^bold>a\<^bold>s\<^bold>t x \<tycolon> N \<longmapsto> X \<tycolon> (\<^bold>s\<^bold>o\<^bold>m\<^bold>e N)" unfolding Cast_def by auto
 lemma someE_\<nu>cast[\<nu>cast_overload E]: "\<^bold>c\<^bold>a\<^bold>s\<^bold>t X \<tycolon> (\<^bold>s\<^bold>o\<^bold>m\<^bold>e N) \<longmapsto> (\<exists>*some. \<tort_lbrace>some \<tycolon> N \<tort_rbrace> \<addition> (some \<in> X))" unfolding Cast_def by auto
+
+subsubsection \<open>Pointer'\<close>
+
+definition "Pointer' = Pointer \<^bold>w\<^bold>h\<^bold>e\<^bold>r\<^bold>e {x. pred_owning within_mem x}"
+
+lemma [simp]: "memadr i' \<nuLinkL> Pointer' \<nuLinkR> i \<longleftrightarrow> (i' = i) \<and> pred_owning within_mem i" unfolding Pointer'_def by auto
+lemma [elim]: "z \<left_fish_tail> i \<ratio> Pointer' \<Longrightarrow> (within_mem i \<Longrightarrow> C) \<Longrightarrow> C" and [elim]: "\<down_fish_tail> \<ratio> Pointer' \<Longrightarrow> C \<Longrightarrow> C"
+  unfolding Inhabited_def by (simp add: memadr_exisits)+
+
+subsubsection \<open>Reference\<close>
+
+definition "Ref N = \<lbrace> Pointer' \<nuFusion> MemObj N \<rbrace>
+  <down-lift> (\<lambda>x. case x of (zp \<left_fish_tail> a \<R_arr_tail> z \<left_fish_tail> x) \<Rightarrow> (zp \<left_fish_tail> a, z \<left_fish_tail> a \<R_arr_tail> x) | (zp \<left_fish_tail> a \<R_arr_tail> \<down_fish_tail>) \<Rightarrow> (zp \<left_fish_tail> a, \<down_fish_tail>) | \<down_fish_tail> \<Rightarrow> (\<down_fish_tail>,\<down_fish_tail>))"
+
+lemma [simp]: "p \<nuLinkL> Ref N \<nuLinkR> (zp \<left_fish_tail> a \<R_arr_tail> z \<left_fish_tail> x) \<longleftrightarrow> p \<nuLinkL> \<lbrace> Pointer' \<nuFusion> MemObj N \<rbrace> \<nuLinkR> (zp \<left_fish_tail> a, z \<left_fish_tail> a \<R_arr_tail> x)"
+  and [simp]: "p \<nuLinkL> Ref N \<nuLinkR> (zp \<left_fish_tail> a \<R_arr_tail> \<down_fish_tail>) \<longleftrightarrow> p \<nuLinkL> \<lbrace> Pointer' \<nuFusion> MemObj N \<rbrace> \<nuLinkR> (zp \<left_fish_tail> a, \<down_fish_tail>)"
+  and [simp]: "p \<nuLinkL> Ref N \<nuLinkR> \<down_fish_tail> \<longleftrightarrow> p \<nuLinkL> \<lbrace> Pointer' \<nuFusion> MemObj N \<rbrace> \<nuLinkR> (\<down_fish_tail>, \<down_fish_tail>)"
+  unfolding Ref_def by simp+
+
+definition "share_ref z x = (case x of (zp \<left_fish_tail> a \<R_arr_tail> zx \<left_fish_tail> x) \<Rightarrow> (zp + z \<left_fish_tail> a \<R_arr_tail> zx + z \<left_fish_tail> x) | (zp \<left_fish_tail> a \<R_arr_tail> \<down_fish_tail>) \<Rightarrow> (zp + z \<left_fish_tail> a \<R_arr_tail> \<down_fish_tail>) | \<down_fish_tail> \<Rightarrow> \<down_fish_tail>)"
+lemma [simp]: "share_ref z (zp \<left_fish_tail> a \<R_arr_tail> zx \<left_fish_tail> x) = (zp + z \<left_fish_tail> a \<R_arr_tail> zx + z \<left_fish_tail> x)"
+  and [simp]: "share_ref z (zp \<left_fish_tail> a \<R_arr_tail> \<down_fish_tail>) = (zp + z \<left_fish_tail> a \<R_arr_tail> \<down_fish_tail>)"
+  and [simp]: "share_ref z \<down_fish_tail> = \<down_fish_tail>"
+  unfolding share_ref_def by auto
+lemma [\<nu>intro]: "\<nu>Share (Ref N) (\<lambda>x. T) share_ref"
+  unfolding \<nu>Share_def by (simp add: tuple_forall object_forall owning_forall memadr_forall memcon_forall)
+
 
 (* section \<open>Others\<close>
 
